src/single_conf_message/DY.Example.SingleConfMessage.Protocol.Stateful.Proof.fst
@@ -34,7 +34,7 @@ let event_predicate_protocol: event_predicate single_message_event =
     | SenderSendMsg sender receiver msg -> True
     | ReceiverReceivedMsg receiver msg -> (
       (exists sender. is_knowable_by (comm_label sender receiver) tr msg.secret) /\
-      event_triggered tr receiver (CommConfReceiveMsg receiver (serialize single_message msg))
+      event_triggered tr receiver (CommConfReceiveMsg receiver msg <: communication_core_event single_message)
     )
 
 let all_sessions = [
@@ -45,13 +45,13 @@ let all_sessions = [
 
 /// List of all local event predicates.
 
-// This is just a demonstration how to use the `comm_higher_layer_event_preds`.
+// This is just a demonstration how to use the `comm_core_higher_layer_event_preds`.
 // If you don't need them you can just initialize them with
-// `default_comm_higher_layer_event_preds`.
+// `default_comm_core_higher_layer_event_preds`.
 #push-options "--fuel 0 --ifuel 2"
-val comm_layer_event_preds: comm_higher_layer_event_preds single_message
+val comm_layer_event_preds: comm_core_higher_layer_event_preds single_message
 let comm_layer_event_preds = {
-  default_comm_higher_layer_event_preds single_message with
+  default_comm_core_higher_layer_event_preds single_message with
   send_conf = (fun tr sender receiver (payload:single_message) ->
     event_triggered tr sender (SenderSendMsg sender receiver payload) /\
 
@@ -71,7 +71,7 @@ let comm_layer_event_preds = {
 #pop-options
 
 let all_events = [
-  event_predicate_communication_layer_and_tag comm_layer_event_preds;
+  event_predicate_communication_layer_core_and_tag comm_layer_event_preds;
   mk_event_tag_and_pred event_predicate_protocol
 ]
 
@@ -90,7 +90,12 @@ instance protocol_invariants_protocol: protocol_invariants = {
 /// Lemmas that the global predicates contain all the local ones
 
 let _ = do_split_boilerplate mk_state_pred_correct all_sessions
-let _ = do_split_boilerplate mk_event_pred_correct all_events
+#push-options "--fuel 2"
+let _ = (
+  assert_norm(List.Tot.no_repeats_p (List.Tot.map fst (all_events)));
+  do_split_boilerplate mk_event_pred_correct all_events
+)
+#pop-options
 
 (*** Proofs ***)
 
